PropositionalLogic/DeepEmbedded/Completeness.v
@@ -13,6 +13,7 @@ Require Import Logic.PropositionalLogic.ProofTheory.Intuitionistic.
 Require Import Logic.PropositionalLogic.ProofTheory.DeMorgan.
 Require Import Logic.PropositionalLogic.ProofTheory.GodelDummett.
 Require Import Logic.PropositionalLogic.ProofTheory.Classical.
+Require Import Logic.SeparationLogic.ProofTheory.SeparationLogic.
 Require Import Logic.PropositionalLogic.Semantics.Trivial.
 Require Import Logic.PropositionalLogic.Semantics.Kripke.
 Require Import Logic.PropositionalLogic.Complete.ContextProperty_Kripke.
