SeparationLogic/Complete/Lindenbaum_Flat.v
@@ -1,0 +1,204 @@
+Require Import Coq.Logic.FunctionalExtensionality.
+Require Import Coq.Logic.Classical_Prop.
+Require Import Coq.Logic.Classical_Pred_Type.
+Require Import Logic.lib.Bijection.
+Require Import Logic.lib.Countable.
+Require Import Logic.GeneralLogic.Base.
+Require Import Logic.GeneralLogic.HenkinCompleteness.
+Require Import Logic.GeneralLogic.KripkeModel.
+Require Import Logic.MinimunLogic.Syntax.
+Require Import Logic.PropositionalLogic.Syntax.
+Require Import Logic.SeparationLogic.Syntax.
+Require Import Logic.MinimunLogic.ProofTheory.Normal.
+Require Import Logic.MinimunLogic.ProofTheory.Minimun.
+Require Import Logic.MinimunLogic.ProofTheory.ContextProperty.
+Require Import Logic.PropositionalLogic.ProofTheory.Intuitionistic.
+Require Import Logic.PropositionalLogic.ProofTheory.DeMorgan.
+Require Import Logic.PropositionalLogic.ProofTheory.GodelDummett.
+Require Import Logic.PropositionalLogic.ProofTheory.Classical.
+Require Import Logic.PropositionalLogic.ProofTheory.RewriteClass.
+Require Import Logic.SeparationLogic.ProofTheory.SeparationLogic.
+Require Import Logic.SeparationLogic.ProofTheory.RewriteClass.
+Require Import Logic.SeparationLogic.ProofTheory.DerivedRules.
+
+Local Open Scope logic_base.
+Local Open Scope syntax.
+Import PropositionalLanguageNotation.
+Import SeparationLogicNotation.
+
+Section Lindenbaum_Flat.
+
+Context {L: Language}
+        {nL: NormalLanguage L}
+        {pL: PropositionalLanguage L}
+        {sL: SeparationLanguage L}
+        {Gamma: ProofTheory L}
+        {nGamma: NormalProofTheory L Gamma}
+        {mpGamma: MinimunPropositionalLogic L Gamma}
+        {ipGamma: IntuitionisticPropositionalLogic L Gamma}
+        {sGamma: SeparationLogic L Gamma}.
+
+Hypothesis CE: Countable expr.
+
+Lemma Lindenbaum_lemma_right:
+  forall Phi1 Phi2 Phi,
+    (forall x y, Phi1 |-- x -> Phi |-- y -> Phi2 |-- x * y) ->
+    (derivable_closed Phi2 /\ orp_witnessed Phi2 /\ consistent Phi2) ->
+    exists Psi,
+      Included _ Phi Psi /\
+      (forall x y, Phi1 |-- x -> Psi |-- y -> Phi2 |-- x * y) /\
+      derivable_closed Psi /\
+      orp_witnessed Psi /\
+      consistent Psi.
+Proof.
+  intros ? ? ? ? [Phi2_DC [Phi2_OW Phi2_C]].
+  set (step :=
+          fun n Phi x0 =>
+             Phi x0 \/
+            (CE x0 n /\
+             (forall x y, Phi1 |-- x -> Phi |-- x0 --> y -> Phi2 |-- x * y))).
+  exists (LindenbaumConstruction step Phi).
+  assert (Included expr Phi (LindenbaumConstruction step Phi) /\
+          (forall x y,
+            Phi1 |-- x ->
+            LindenbaumConstruction step Phi |-- y ->
+            Phi2 |-- x * y) /\
+          ((forall x y,
+            Phi1 |-- x ->
+            LindenbaumConstruction step Phi |-- y ->
+            Phi2 |-- x * y) ->
+           derivable_closed (LindenbaumConstruction step Phi)) /\
+          ((forall x y,
+            Phi1 |-- x ->
+            LindenbaumConstruction step Phi |-- y ->
+            Phi2 |-- x * y) ->
+           orp_witnessed (LindenbaumConstruction step Phi)) /\
+          ((forall x y,
+            Phi1 |-- x ->
+            LindenbaumConstruction step Phi |-- y ->
+            Phi2 |-- x * y) ->
+           consistent (LindenbaumConstruction step Phi))).
+  Focus 2. {
+    destruct H0 as [? [? [? [? ?]]]].
+    split; [| split; [| split; [| split]]]; auto.
+  } Unfocus.
+  split; [| split; [| split; [| split]]].
+  + apply (Lindenbaum_spec_included _ _ 0).
+  + intros.
+    apply NNPP.
+    intro; revert H1.
+    apply (Lindenbaum_spec_pos _ _
+            (fun xs => |-- multi_imp xs y)
+            (fun Phi => Phi |-- y)).
+    - intros; apply derivable_provable.
+    - intros ? ? ? ?; left; auto.
+    - intro; apply H2; clear H2.
+      apply (H x y); auto.
+    - intros.
+      destruct (Classical_Prop.classic (exists y0, CE y0 n /\ (forall x y, Phi1 |-- x -> S |-- y0 --> y -> Phi2 |-- x * y))) as [[y0 [? ?]] |].
+      * intro; apply H2; clear H2.
+        specialize (H4 _ y H0).
+        apply H4; clear H4.
+        rewrite <- deduction_theorem.
+        eapply deduction_weaken; [| exact H5].
+        hnf; intros ? [? | [? ?]]; [left; auto |].
+        pose proof in_inj _ _ CE _ _ _ H2 H3.
+        subst; right; constructor.
+      * intro; apply H1; clear H1.
+        eapply deduction_weaken; [| exact H4].
+        hnf; intros ? [? | [? ?]]; [auto |].
+        exfalso; apply H3; clear H3.
+        exists x0; auto.
+  + intros; hnf; intros.
+    destruct (im_inj _ _ CE x) as [n ?].
+    apply (Lindenbaum_spec_neg _ _ _ (S n)).
+    simpl.
+    unfold step at 1.
+    right; split; auto.
+    intros.
+    eapply deduction_weaken in H4; [| apply (Lindenbaum_spec_included _ _ n)].
+    pose proof deduction_modus_ponens _ _ _ H1 H4.
+    auto.
+  + intros; hnf; intros x0 y0 ?.
+    destruct (im_inj _ _ CE x0) as [nx ?].
+    destruct (im_inj _ _ CE y0) as [ny ?].
+    assert (LindenbaumChain step Phi (S nx) x0 \/ LindenbaumChain step Phi (S ny) y0) as HH;
+      [| destruct HH as [HH | HH]; apply Lindenbaum_spec_neg in HH; auto].
+    simpl.
+    unfold step at 1 3.
+    assert ((forall x y,
+              Phi1 |-- x ->
+              LindenbaumChain step Phi nx |-- x0 --> y ->
+              Phi2 |-- x * y) \/
+            (forall x y,
+              Phi1 |-- x ->
+              LindenbaumChain step Phi ny |-- y0 --> y ->
+              Phi2 |-- x * y)) as HH;
+      [| destruct HH as [HH | HH]; auto].
+    assert ((forall x y,
+              Phi1 |-- x ->
+              LindenbaumConstruction step Phi |-- x0 --> y ->
+              Phi2 |-- x * y) \/
+            (forall x y,
+              Phi1 |-- x ->
+              LindenbaumConstruction step Phi |-- y0 --> y ->
+              Phi2 |-- x * y)) as HH;
+      [
+      | destruct HH as [HH | HH]; [left | right];
+        intros xx yy ? ?; apply (HH xx yy); auto;
+        eapply deduction_weaken;
+        [apply (Lindenbaum_spec_included _ _ nx) | auto
+        |apply (Lindenbaum_spec_included _ _ ny) | auto ]].
+
+    clear nx ny H2 H3.
+    apply NNPP.
+    intro.
+    apply Classical_Prop.not_or_and in H2; destruct H2.
+    apply Classical_Pred_Type.not_all_ex_not in H2.
+    apply Classical_Pred_Type.not_all_ex_not in H3.
+    destruct H2 as [x'' ?], H3 as [y'' ?].
+    apply Classical_Pred_Type.not_all_ex_not in H2.
+    apply Classical_Pred_Type.not_all_ex_not in H3.
+    destruct H2 as [x' ?], H3 as [y' ?].
+    apply imply_to_and in H2.
+    apply imply_to_and in H3.
+    destruct H2, H3.
+    apply imply_to_and in H4.
+    apply imply_to_and in H5.
+    destruct H4, H5.
+
+    rewrite <- deduction_theorem in H4.
+    apply (deduction_orp_intros1 _ _ y') in H4.
+    rewrite deduction_theorem in H4.
+    rewrite <- deduction_theorem in H5.
+    apply (deduction_orp_intros2 _ x') in H5.
+    rewrite deduction_theorem in H5.
+    pose proof deduction_orp_elim _ _ _ _ H4 H5.
+    pose proof deduction_modus_ponens _ _ _ (derivable_assum _ _ H1) H8.
+    pose proof deduction_andp_intros _ _ _ H2 H3.
+    clear H2 H3 H4 H5 H8.
+    pose proof H0 _ _ H10 H9.
+    pose proof derivable_sepcon_orp_right Phi2 (x'' && y'') x' y'.
+    apply deduction_andp_elim1 in H3.
+    pose proof deduction_modus_ponens _ _ _ H2 H3.
+    rewrite <- derivable_closed_element_derivable in H4 by auto.
+    apply Phi2_OW in H4.
+    rewrite !(derivable_closed_element_derivable Phi2) in H4 by auto.
+    clear H10 H2 H3.
+    destruct H4.
+    - pose proof derivable_sepcon_andp_left Phi2 x'' y'' x'.
+      pose proof deduction_modus_ponens _ _ _ H2 H3.
+      apply deduction_andp_elim1 in H4; auto.
+    - pose proof derivable_sepcon_andp_left Phi2 x'' y'' y'.
+      pose proof deduction_modus_ponens _ _ _ H2 H3.
+      apply deduction_andp_elim2 in H4; auto.
+  + intros.
+    rewrite consistent_spec in Phi2_C |- *; intro.
+    pose proof derivable_impp_refl Phi1 FF.
+    specialize (H0  _ _ H2 H1).
+    pose proof derivable_sepcon_FF Phi2 TT.
+    pose proof deduction_modus_ponens _ _ _ H0 H3.
+    auto.
+Qed.
+
+End Lindenbaum_Flat.
