SeparationLogic/DeepEmbedded/ParametricCompletenss.v
@@ -1,0 +1,202 @@
+Require Import Coq.Logic.Classical_Prop.
+Require Import Logic.lib.Ensembles_ext.
+Require Import Logic.lib.Bijection.
+Require Import Logic.lib.Countable.
+Require Import Logic.GeneralLogic.Base.
+Require Import Logic.MinimunLogic.Syntax.
+Require Import Logic.PropositionalLogic.Syntax.
+Require Import Logic.SeparationLogic.Syntax.
+Require Import Logic.MinimunLogic.ProofTheory.Normal.
+Require Import Logic.MinimunLogic.ProofTheory.Minimun.
+Require Import Logic.MinimunLogic.ProofTheory.ContextProperty.
+Require Import Logic.PropositionalLogic.ProofTheory.Intuitionistic.
+Require Import Logic.PropositionalLogic.ProofTheory.DeMorgan.
+Require Import Logic.PropositionalLogic.ProofTheory.GodelDummett.
+Require Import Logic.PropositionalLogic.ProofTheory.Classical.
+Require Import Logic.SeparationLogic.ProofTheory.SeparationLogic.
+Require Import Logic.SeparationLogic.ProofTheory.RewriteClass.
+Require Import Logic.SeparationLogic.ProofTheory.DerivedRules.
+Require Import Logic.GeneralLogic.KripkeModel.
+Require Import Logic.SeparationLogic.Model.SeparationAlgebra.
+Require Import Logic.SeparationLogic.Model.OrderedSA.
+Require Import Logic.PropositionalLogic.Semantics.Kripke.
+Require Import Logic.SeparationLogic.Semantics.FlatSemantics.
+Require Import Logic.PropositionalLogic.Complete.ContextProperty_Kripke.
+Require Import Logic.PropositionalLogic.Complete.Lindenbaum_Kripke.
+Require Import Logic.PropositionalLogic.Complete.Truth_Kripke.
+Require Import Logic.PropositionalLogic.Complete.Canonical_Kripke.
+Require Import Logic.PropositionalLogic.Complete.Complete_Kripke.
+Require Import Logic.SeparationLogic.Complete.ContextProperty_Flat.
+Require Import Logic.SeparationLogic.Complete.Lindenbaum_Flat.
+Require Import Logic.SeparationLogic.Complete.Truth_Flat.
+Require Import Logic.SeparationLogic.Complete.Canonical_Flat.
+Require Import Logic.SeparationLogic.DeepEmbedded.Parameter.
+Require Logic.SeparationLogic.DeepEmbedded.SeparationEmpLanguage.
+Require Logic.SeparationLogic.DeepEmbedded.FlatSemantics.
+Require Logic.SeparationLogic.DeepEmbedded.ParametricSeparationLogic.
+
+Local Open Scope logic_base.
+Local Open Scope syntax.
+Local Open Scope kripke_model.
+Local Open Scope kripke_model_class.
+Import PropositionalLanguageNotation.
+Import SeparationLogicNotation.
+Import KripkeModelFamilyNotation.
+Import KripkeModelNotation_Intuitionistic.
+Import KripkeModelClass.
+
+Section Complete.
+
+Context (Var: Type).
+Context (CV: Countable Var).
+Context (SLP: SL_Parameter).
+
+Instance L: Language := SeparationEmpLanguage.L Var.
+Instance nL: NormalLanguage L := SeparationEmpLanguage.nL Var.
+Instance pL: PropositionalLanguage L := SeparationEmpLanguage.pL Var.
+Instance sL: SeparationLanguage L := SeparationEmpLanguage.sL Var.
+Instance s'L: SeparationEmpLanguage L := SeparationEmpLanguage.s'L Var.
+
+Instance G: ProofTheory L := ParametricSeparationLogic.G Var SLP.
+Instance nG: NormalProofTheory L G := ParametricSeparationLogic.nG Var SLP.
+Instance mpG: MinimunPropositionalLogic L G := ParametricSeparationLogic.mpG Var SLP.
+Instance ipG: IntuitionisticPropositionalLogic L G := ParametricSeparationLogic.ipG Var SLP.
+Instance sG: SeparationLogic L G := ParametricSeparationLogic.sG Var SLP.
+Instance eG: EmpSeparationLogic L G := ParametricSeparationLogic.eG Var SLP.
+Instance ParG: ParametricSeparationLogic.Parametric_SeparationLogic SLP L G := ParametricSeparationLogic.ParG Var SLP.
+
+Instance MD: Model := FlatSemantics.MD Var.
+Instance kMD: KripkeModel MD := FlatSemantics.kMD Var.
+Instance R (M: Kmodel): Relation (Kworlds M):= FlatSemantics.R Var M.
+Instance J (M: Kmodel): Join (Kworlds M):= FlatSemantics.J Var M.
+
+Instance SM: Semantics L MD := FlatSemantics.SM Var.
+Instance kpSM (M: Kmodel): KripkePropositionalSemantics L MD M SM := FlatSemantics.kpSM Var M.
+Instance fsSM (M: Kmodel): FlatSemantics.SeparatingSemantics L MD M SM := FlatSemantics.fsSM Var M.
+Instance feSM (M: Kmodel): FlatSemantics.EmpSemantics L MD M SM := FlatSemantics.feSM Var M.
+
+Definition DDC: context -> Prop := fun Psi =>
+  derivable_closed Psi /\ orp_witnessed Psi /\ consistent Psi.
+
+Lemma DER: at_least_derivable_closed DDC.
+Proof. hnf; intros ? [? [? ?]]; auto. Qed.
+
+Lemma ORP: at_least_orp_witnessed DDC.
+Proof. hnf; intros ? [? [? ?]]; auto. Qed.
+
+Lemma CONSI: at_least_consistent DDC.
+Proof. hnf; intros ? [? [? ?]]; auto. Qed.
+
+Lemma LIN_DER: Linderbaum_derivable DDC.
+Proof.
+  hnf; intros.
+  pose proof Lindenbaum_lemma
+    (SeparationEmpLanguage.formula_countable Var CV) _ _ H
+  as [Psi [? [? ?]]].
+  exists (exist _ Psi H2); auto.
+Qed.
+
+Lemma LIN_SR: Linderbaum_sepcon_right DDC.
+Proof.
+  hnf; intros.
+  pose proof Lindenbaum_lemma_right
+    (SeparationEmpLanguage.formula_countable Var CV) _ _  _ H (proj2_sig Psi)
+  as [Psi2 [? [? ?]]].
+  exists (exist _ Psi2 H2); auto.
+Qed.
+
+Lemma LIN_SL: Linderbaum_sepcon_left DDC.
+Proof. rewrite Linderbaum_sepcon_equiv. apply LIN_SR. Qed.
+
+Definition canonical_frame: FlatSemantics.frame :=
+  FlatSemantics.Build_frame (sig DDC)
+    (fun a b => Included _ (proj1_sig a) (proj1_sig b))
+    (fun a b c => context_join (proj1_sig a) (proj1_sig b) (proj1_sig c)).
+
+Definition canonical_eval: Var -> FlatSemantics.sem canonical_frame :=
+  fun p a => proj1_sig a (SeparationEmpLanguage.varp p).
+
+Definition canonical_Kmodel: @Kmodel (FlatSemantics.MD Var) (FlatSemantics.kMD Var) :=
+  FlatSemantics.Build_Kmodel Var canonical_frame canonical_eval.
+
+Definition rel: bijection (Kworlds canonical_Kmodel) (sig DDC) := bijection_refl.
+
+Definition H_R:
+  forall m n Phi Psi, rel m Phi -> rel n Psi ->
+    (m <= n <-> Included _ (proj1_sig Phi) (proj1_sig Psi)).
+Proof.
+  intros.
+  change (m = Phi) in H.
+  change (n = Psi) in H0.
+  subst; reflexivity.
+Qed.
+
+Definition H_J:
+  forall m1 m2 m Phi1 Phi2 Phi, rel m1 Phi1 -> rel m2 Phi2 -> rel m Phi ->
+    (join m1 m2 m <-> context_join (proj1_sig Phi1) (proj1_sig Phi2) (proj1_sig Phi)).
+Proof.
+  intros.
+  change (m = Phi) in H1.
+  change (m1 = Phi1) in H.
+  change (m2 = Phi2) in H0.
+  subst; reflexivity.
+Qed.
+
+Lemma TRUTH:
+  forall x: expr, forall m Phi, rel m Phi ->
+    (KRIPKE: canonical_Kmodel, m |= x <-> proj1_sig Phi x).
+Proof.
+  induction x.
+  + exact (truth_lemma_andp DDC rel DER x1 x2 IHx1 IHx2).
+  + exact (truth_lemma_orp DDC rel DER ORP x1 x2 IHx1 IHx2).
+  + exact (truth_lemma_impp DDC rel H_R DER LIN_DER x1 x2 IHx1 IHx2).
+  + exact (truth_lemma_sepcon DDC rel H_J DER LIN_SL LIN_SR x1 x2 IHx1 IHx2).
+  + exact (truth_lemma_wand DDC rel H_J DER LIN_DER LIN_SR x1 x2 IHx1 IHx2).
+  + exact (truth_lemma_emp DDC rel H_R H_J DER LIN_DER LIN_SR).
+  + exact (truth_lemma_falsep DDC rel CONSI).
+  + intros; change (m = Phi) in H; subst; reflexivity.
+Qed.
+
+Context (SAP: SA_Parameter).
+
+Hypothesis PC: Parameter_coincide SLP SAP.
+
+Theorem ParametricCompleteness:
+  strongly_complete G SM
+    (KripkeModelClass _
+      (FlatSemantics.Kmodel_Monotonic +
+       FlatSemantics.Kmodel_PreOrder +
+       FlatSemantics.Kmodel_SeparationAlgebra +
+       FlatSemantics.Kmodel_UpwardsClosed +
+       FlatSemantics.Kmodel_DownwardsClosed +
+       FlatSemantics.Kmodel_Unital +
+       FlatSemantics.Parametric_Kmodel_Class SAP)).
+Proof.
+  apply (@general_completeness _ _ _ _ _ _ _ _ _ _ DDC rel LIN_DER DER TRUTH).
+  split; [split; [split; [split; [split; [split |] |] |] |] |].
+  + hnf; intros.
+    exact (denote_monotonic DDC rel H_R
+             (SeparationEmpLanguage.varp v)
+             (TRUTH (SeparationEmpLanguage.varp v))).
+  + exact (po_R DDC rel H_R).
+  + exact (SA DDC rel H_J LIN_SR).
+  + exact (uSA DDC rel H_R H_J DER).
+  + exact (dSA DDC rel H_R H_J DER).
+  + exact (unitSA DDC rel H_R H_J DER LIN_SR TRUTH).
+  + inversion PC.
+    constructor; intros HH; rewrite HH in *.
+    - pose proof ParametricSeparationLogic.Parametric_C H.
+      exact (classical_canonical_ident DDC rel H_R DER ORP CONSI).
+    - pose proof ParametricSeparationLogic.Parametric_GD H0.
+      exact (GodelDummett_canonical_no_branch DDC rel H_R DER ORP).
+    - pose proof ParametricSeparationLogic.Parametric_DM H1.
+      exact (DeMorgan_canonical_branch_join DDC rel H_R DER ORP CONSI LIN_DER).
+    - pose proof ParametricSeparationLogic.Parametric_GC H2.
+      exact (garbage_collected_canonical_increaing DDC rel H_R H_J DER).
+    - pose proof ParametricSeparationLogic.Parametric_NE H3.
+      exact (nonsplit_canonical_split_smaller DDC rel H_R H_J DER TRUTH).
+    - pose proof ParametricSeparationLogic.Parametric_ED H4.
+      exact (dup_canonical_incr_join DDC rel H_J DER TRUTH).
+Qed.
+
+End Complete.
